examples/crypto/HyE.PlainAE.fst
@@ -6,34 +6,44 @@ open HyE.Indexing
 open HyE.PlainHPKE
 open Platform.Bytes
 
+module B = Platform.Bytes
 
 (**
-   The content of the AE payload depends on the honesty of the message.
-   If it is an honest message, it encapsulates a (protected) hpke payload.
-   If it is not an honest message, it is plain bytes.
+   If we give guarantees for hpke and the plaintext is pke_honest, 
+   but not ae_honest, then we do not protect it on hpke_level. On
+   the other hand, if we do not give guarantees on the pke level or
+   the plaintext is not pke_honest, we can "protect" it and call repr.
+   This allows us to avoid branching on the pke_honesty of the plaintext
+   in HPKE.encrypt.
 *)
-abstract type protected_ae_plain (i:ae_id) = (
-  if pke_honest (fst i) && not (ae_honest i) && hpke_ind_cca then
-    protected_hpke_plain (fst i)
-  else 
+type protected_ae_plain (i:ae_id) = (
+  if (pke_honest (fst i) && hpke_ind_cca) && not (ae_honest i && ae_ind_cca) then
     hpke_plain
+  else 
+    protected_hpke_plain (fst i)
   )
 
-type ae_plain = Bytes.bytes
+type ae_plain = B.bytes
 
 val length: #i:ae_id -> (protected_ae_plain i) -> Tot nat
 let length #i p = 
-  if pke_honest (fst i) && not (ae_honest i) && hpke_ind_cca then
-    PlainHPKE.length p
+  if (pke_honest (fst i) && hpke_ind_cca) && not (ae_honest i && ae_ind_cca) then
+    B.length p
   else
-    Bytes.length p
+    PlainHPKE.length #(fst i) p
+
 
 (**
-   Coerced messages can only be flagged as not honest.
+   Coerced messages can only be flagged as not honest. The if condition reflects the
+   dependent nature of the protected_ae_plain type. If we have protection on the
+   HPKE level, we have to call coerce.
 *)
 val coerce: #i:ae_id -> p:ae_plain{not ae_ind_cca || not (ae_honest i)} -> Tot (protected_ae_plain i)
 let coerce #i p = 
-  p
+  if (pke_honest (fst i) && hpke_ind_cca) && not (ae_honest i && ae_ind_cca) then
+    p
+  else 
+    PlainHPKE.coerce #(fst i) p
 
 (**
    We allow a transition from protected_ae_plain to ae_plain only if either there is no
@@ -41,33 +51,15 @@ let coerce #i p =
 *)
 val repr: #i:ae_id -> p:protected_ae_plain i{not ae_ind_cca || not (ae_honest i)} -> Tot (ae_plain)
 let repr #i p = 
-  if ae_honest i && ae_ind_cca then
-    PlainHPKE.repr p.p 
-  else
-    p.p
-//
-//(**
-//   This is a helper function used by HPKE.encrypt to encapsulate the payload before
-//   passing it on to AE.encrypt. If AE is idealized and the payload is honest, then we 
-//   wrap the payload into our abstract type in good faith. If not, we coerce it.
-//*)
-//val ae_message_wrap: #i:ae_id -> p:protected_ae_plain i -> Tot (protected_ae_plain i)
-//let ae_message_wrap #i p =
-//  if ae_honest i && ae_ind_cca then
-//    Protected_ae_plain p
-//  else
-//    coerce p
-//
-//(**
-//   This is the reverse function to ae_message_wrap. HPKE.decrypt uses it to extract a
-//   protected ae payload. If it AE is idealized and the payload is honest, then
-//   we strip it of its protection in good faith. Otherwise we break it down to its 
-//   byte representation using repr.
-//*)
-//val ae_message_unwrap: #i:ae_id -> p:protected_ae_plain i -> Tot (ae_plain_content i)
-//let ae_message_unwrap #i p =
-//  if ae_honest i && ae_ind_cca then
-//    p.p
-//  else 
-//repr p
+  if (pke_honest (fst i) && hpke_ind_cca) && not (ae_honest i && ae_ind_cca) then
+    p
+  else 
+    PlainHPKE.repr #(fst i) p
 
+val ae_unwrap: #i:ae_id -> protected_ae_plain i -> Tot (protected_hpke_plain (fst i))
+let ae_unwrap #i p =
+  if (pke_honest (fst i) && hpke_ind_cca) && not (ae_honest i && ae_ind_cca) then
+    PlainHPKE.coerce #(fst i) p
+  else 
+    p
+  
