examples/crypto/HyE.PlainHPKE.fst
@@ -11,7 +11,9 @@ open Platform.Bytes
 open HyE.Flags
 open HyE.Indexing
 
-type hpke_plain = Bytes.bytes
+module B = Platform.Bytes
+
+type hpke_plain = B.bytes
 
 abstract type protected_hpke_plain (i:pke_id) = hpke_plain
 
@@ -20,9 +22,9 @@ val repr: #i:pke_id -> p:protected_hpke_plain i{not (pke_honest i) || not hpke_i
 let repr #i p = p
 
 // Change this if we want to use signcryption with hpke_int-ctxt
-val coerce: #i:pke_id -> p:hpke_plain{not (pke_honest i) || not hpke_ind_cca} -> Tot (protected_hpke_plain i)
-let coerce #i p = 
+val coerce: #i:pke_id -> p:hpke_plain -> Tot (protected_hpke_plain i)
+let coerce #i p =
   p
 
 val length: #i:pke_id -> protected_hpke_plain i -> Tot nat
-let length #i p = Bytes.length p
+let length #i p = B.length p
