examples/crypto/HyE.PlainPKE.fst
@@ -7,22 +7,20 @@ open Platform.Bytes
 open HyE.RSA
 open HyE.Flags
 open HyE.AE
-open HyE.PlainAE
 open HyE.Indexing
 open FStar.HyperHeap
 open FStar.HyperStack
 open FStar.Monotonic.RRef
 
-noeq type protected_pke_plain (i:pke_id) =
-  | Prot_pke_plain : k:AE.key{fst (get_index k) = i} -> protected_pke_plain i
+type protected_pke_plain (i:pke_id) = k:AE.key{i= fst (get_index k)}
 
 type pke_plain (i:pke_id) = aes_key 
 
 (* two pure functions, never called when ideal *)
 val repr: #i:pke_id -> p:protected_pke_plain i{not pke_ind_cca || not (pke_honest i)} -> Tot (pke_plain i)
-let repr #i p = HyE.AE.leak_key #(AE.get_index p.k) p.k
+let repr #i p = HyE.AE.leak_key #(AE.get_index p) p
 
 // Not sure how the ids are supposed to work with coerce...
-val coerce: #num:UInt32.t -> #i:pke_id{not (ae_honest (i,num))} -> parent:rid -> pke_plain i -> St (protected_pke_plain i)
-let coerce #num #i parent p_plain = 
-  Prot_pke_plain (HyE.AE.coerce_key (i,num) parent p_plain)
+val coerce: #i:ae_id{not (ae_honest i) || not ae_ind_cca} -> parent:rid -> pke_plain (fst i) -> St (p:protected_pke_plain (fst i))
+let coerce #i parent p_plain = 
+  HyE.AE.coerce_key i parent p_plain
