examples/crypto/HyE.Indexing.fsti
@@ -10,7 +10,8 @@ val ae_honest: i:ae_id -> Tot (b:bool{b ==> pke_honest (fst i)})
 
 val fresh_pke_id: unit -> Tot (i:pke_id{pke_honest i})
 
-val fresh_ae_id: pk_id:pke_id -> Tot (k_id:ae_id{fst k_id = pk_id})
-val dishonest_ae_id: pk_i:pke_id -> Tot (k_id:ae_id{not (ae_honest k_id)})
+// TODO: Try typechecking without refinements!
+val fresh_ae_id: pk_id:pke_id -> Tot (k_id:ae_id{fst k_id = pk_id /\ (pke_honest pk_id ==> b2t (ae_honest k_id))})
+val dishonest_ae_id: pk_id:pke_id -> Tot (k_id:ae_id{not (ae_honest k_id) && fst k_id = pk_id})
 
 assume Index_hasEq: hasEq pke_id
